examples/Online_with_authn/DY.OnlineA.Invariants.fst
@@ -24,68 +24,55 @@ open DY.OnlineA.Protocol
 /// With this, we then know that
 /// the protocol model satisfies the secrecy property.
 
+/// We only highlight the differences to the previous model
+/// for showing nonce secrecy.
 
 (*** Crypto Invariants ***)
 
 
-(** TODO **)
-// needed for `crypto_prediates.pke_pred.pred_later`
 %splice [ps_ping_t_is_well_formed] (gen_is_well_formed_lemma (`ping_t))
 %splice [ps_ack_t_is_well_formed] (gen_is_well_formed_lemma (`ack_t))
 %splice [ps_message_t_is_well_formed] (gen_is_well_formed_lemma (`message_t))
 
-
-
-// ignore this for now
 instance crypto_usages_p : crypto_usages = default_crypto_usages
 
 #push-options "--ifuel 2"
 let crypto_p : crypto_predicates = { 
   default_crypto_predicates with 
-  (* we restrict when a message is allowed to be encrypted 
-     with some secret key
-
-     Or put differently:
-     What are the guarantees that an honest sender can provide
-     that are available at the receiver after decryption?
-  *)
   pke_pred = { 
     pred = (fun tr sk_usage msg ->
-    exists prin. // the intended receiver of the message
+    exists prin.
     (
-      // needed for `decode_ping_proof` [Why?]
-      (* the key used for the encryption is
-         a protocol-level public key for the intended receiver (prin) 
-      *)
       sk_usage == long_term_key_type_to_usage (LongTermPkeKey key_tag) prin /\
       (match parse message_t msg with
       | Some (Ping ping) ->
-          (* a Ping message can only be encrypted if
-             (Or: if you decrypt a Ping from an honest party 
-             you get the guarantees that:)
-             the contained nonce n_a
-             is labeled for 
-             * the name provided in the message (alice)
-             * and the intended receiver of the message (bob)
-          *)
           let bob = prin in
           let alice = ping.alice in
           let n_a = ping.n_a in
           get_label tr n_a == nonce_label alice bob
+
+          (* We add, that the Alice specified in the Ping message,
+             must have triggered an Initiating event
+             with 
+             * her own name (alice)
+             * the intended receiver of the Ping (bob) and
+             * the nonce n_a in the Ping
+          *)
           /\ event_triggered tr alice (Initiating {alice; bob; n_a})
       | Some (Ack ack) ->
+          (* For nonce secrecy,
+             we didn't have any conditions/guarantees in the Ack case.
+             Now, we add that 
+             some Bob must have triggered a Responding event with
+             * the intended receiver of the Ack (alice)
+             * his own name (bob) and
+             * the nonce (n_a) in the Ack
+          *)
           let alice = prin in
-          (get_label tr ack.n_a) `can_flow tr` public \/
-          exists bob. 
-           //event_triggered tr alice (Initiating {alice; bob; n_a = ack.n_a})
-          event_triggered tr bob (Responding {alice; bob; n_a = ack.n_a})
-      | _ -> False // other messages can not be encrypted
+          exists bob. event_triggered tr bob (Responding {alice; bob; n_a = ack.n_a})
+      | _ -> False
       ))
       ); 
-    (* a lemma guaranteeing:
-       if the predicate specified above holds for some trace tr1
-       it also holds for any extension tr2 of tr1
-    *)
     pred_later = (fun tr1 tr2 pk msg -> 
       parse_wf_lemma message_t (bytes_well_formed tr1) msg
     ) 
@@ -103,48 +90,41 @@ instance crypto_invariants_p: crypto_invariants = {
 
 (*** State Invariant ***)
 
-// TODO
-// Needed for `state_predicate.pred_knowable`
 %splice [ps_sent_ping_t_is_well_formed] (gen_is_well_formed_lemma (`sent_ping_t))
 %splice [ps_sent_ack_t_is_well_formed] (gen_is_well_formed_lemma (`sent_ack_t))
 %splice [ps_received_ack_t_is_well_formed] (gen_is_well_formed_lemma (`received_ack_t))
 %splice [ps_state_t_is_well_formed] (gen_is_well_formed_lemma (`state_t))
 
 #push-options "--ifuel 2 --z3cliopt 'smt.qi.eager_threshold=50'"
-(* We restrict what states are allowed to be stored by principals *)
 let state_predicate_p: local_state_predicate state_t = {
   pred = (fun tr prin sess_id st ->
     match st with
     | SentPing ping -> (
-        (* a SentPing state may only be stored if
-           the stored nonce is labeled for
-           * the storing principal (alice)
-           * the principal stored in the state 
-             (the intended receiver of the Ping: bob)
-        *) 
         let alice = prin in
         let bob = ping.bob in
         let n_a = ping.n_a in
         is_secret (nonce_label alice bob) tr n_a
+        (* We add, that the storing principal (alice),
+           must have triggered an Initiating event with:
+           * her own name
+           * the bob stored in the state and
+           * the nonce stored in the state
+        *)
         /\ event_triggered tr alice (Initiating {alice = alice; bob = bob; n_a = n_a})
     )
     | SentAck ack -> (
-        (* a SentAck state may only be stored if
-           the stored nonce is readable by
-           the storing principal (bob)
-
-           -- this is a condition that must always hold,
-           and is enforced by the `pred_knowable` Lemma.
-        *)
         let bob = prin in
         let alice = ack.alice in
         let n_a = ack.n_a in
         is_knowable_by (principal_label bob) tr n_a
-        /\ (
-          // is_publishable tr n_a \/
-          //  event_triggered tr alice (Initiating {alice; bob; n_a})
-          event_triggered tr bob (Responding {alice; bob; n_a})
-        )
+        (* Additionally, we enforce that
+           the storing principal (bob) 
+           must have triggered e Responding event with:
+           * the stored name (alice)
+           * his own name (bob)
+           * the stored nonce (n_a)
+        *)
+        /\ event_triggered tr bob (Responding {alice; bob; n_a})
     )
     | ReceivedAck rack  -> (
         (* a ReceivedAck state may only be stored if
@@ -157,21 +137,22 @@ let state_predicate_p: local_state_predicate state_t = {
         let bob = rack.bob in
         let n_a = rack.n_a in
         is_secret (nonce_label alice bob) tr n_a
-        // /\ (state_was_set_some_id tr bob (SentAck {alice; n_a})
-         /\ ( event_triggered tr bob (Responding {alice; bob; n_a})
-        \/ (is_corrupt tr (principal_label alice) \/ is_corrupt tr (principal_label bob))
-        )
+
+        (* We add, that if both the storing principal (alice)
+           and the stored principal (bob)
+           are honest,
+           then the stored principal (bob)
+           must have triggered a Responding event with:
+           * the storing principal (alice)
+           * his own name (bob) and
+           * the stored nonce (n_a)
+        *)
+         /\ (  event_triggered tr bob (Responding {alice; bob; n_a})
+            \/ (is_corrupt tr (principal_label alice) \/ is_corrupt tr (principal_label bob))
+           )
     )
   );
-  (* as for encryption we have a lemma guaranteeing:
-     if the state predicate holds on some trace tr1
-     it also holds for any extension tr2 of tr2
-  *)
   pred_later = (fun tr1 tr2 prin sess_id st -> () );
-  (* a lemma guaranteeing that
-     the content of the state to be stored
-     is readable by the storing principal
-  *)
   pred_knowable = (fun tr prin sess_id st -> () );
 }
 #pop-options
@@ -205,7 +186,17 @@ let event_predicate_event_t: event_predicate event_t =
         is_secret (nonce_label alice bob) tr n_a /\
         rand_just_generated tr n_a
     )
-    | Responding {alice; bob; n_a} -> (
+    | Responding resp -> (
+        let alice = resp.alice in
+        let bob = resp.bob in
+        let n_a = resp.n_a in
+        (* A Responding event may only be triggered if,
+           * the triggering principal is the second principal stored in the event (bob)
+           * if the stored nonce n_a has not leaked,
+             then the first stored principal (alice)
+             must have triggered an Initiating event with the same data
+             as the Responding event
+        *)
         prin == bob
         /\ (is_publishable tr n_a
           \/ event_triggered tr alice (Initiating {alice; bob; n_a})
@@ -215,7 +206,6 @@ let event_predicate_event_t: event_predicate event_t =
 
 (*** Trace invariants ***)
 
-// TODO: can this (all_sessions and all_events) be hidden somehow?
 let all_sessions = [
   pki_tag_and_invariant;
   private_keys_tag_and_invariant;
@@ -225,12 +215,6 @@ let all_sessions = [
 /// Now we have an event type
 let all_events = [(event_event_t.tag, compile_event_pred event_predicate_event_t)]
 
-
-/// The final trace invariants
-/// consisting of
-/// * the state invariant and
-/// * the event invariant
-
 let trace_invariants_p: trace_invariants = {
   state_pred = mk_state_pred all_sessions;
   event_pred = mk_event_pred all_events;
@@ -239,11 +223,6 @@ let trace_invariants_p: trace_invariants = {
 
 (*** Protocol Invariants ***)
 
-/// The final protocol invariants
-/// consisting of
-/// * the crypto invariants and
-/// * the trace invariants
-
 instance protocol_invariants_p: protocol_invariants = {
   crypto_invs = crypto_invariants_p;
   trace_invs = trace_invariants_p;
@@ -251,8 +230,6 @@ instance protocol_invariants_p: protocol_invariants = {
 
 
 (*** Helper Lemmas for the Secrecy Proof ***)
-
-// TODO: Can all of this be hidden somehow?
 
 val all_sessions_has_all_sessions: unit -> Lemma (norm [delta_only [`%all_sessions; `%for_allP]; iota; zeta] (for_allP (has_local_bytes_state_predicate) all_sessions))
 let all_sessions_has_all_sessions () =
